Identify the error or errors in this argument that supposedly shows that if $$\forall x (P(x) \vee Q(x))$$ is true then $$\forall x P(x) \vee \forall x Q(x)$$ is true.

|Step|Expression|Reason|
|--|--|--|
|1|$$\forall (P(x) \vee Q(x))$$|Premise|
|2|$$P(c) \vee Q(c)$$|Universal instantiation from (1)|
|3|P(c)|Simplification from (2)|
|4|$$\forall x P(x)$$|Universal generalization from (3)|
|5|Q(c)|Simplification from (2)|
|6|$$\forall x Q(x)$$|Universal generalization from (5)|
|7|$$\forall x (P(x) \vee Q(x))$$|Conjunction from (4) and (6)|

Solution

Step 3 and step 5, can't use Simplification.