Use rules of inference to show that if $$\forall x (P(x) \rightarrow (Q(x) \wedge S(x)))$$ and $$\forall x (P(x) \wedge R(x))$$ are true, then $$\forall x (R(x) \wedge S(x))$$ is true.

Solution

|Step|Expresstion|Reason|
|--|--|--|
|1|$$\forall x (P(x) \rightarrow (Q(x) \wedge S(x)))$$|Premise|
|2|$$P(c) \rightarrow (Q(c) \wedge S(c))$$ for arbitrary c|Universal instantiation from (1)|
|3|$$\forall x (P(x) \wedge R(x))$$|Premise|
|4|$$P(c) \wedge R(c)$$ for arbitrary c|Universal instantiation from (3)|
|5|$$P(c) for arbitrary c|Simplification from (4)|
|6|$$R(c) for arbitrary c|SImplification from (4)|
|7|$$S(c) for arbitrary c|Modus ponens from (4) and (5)|
|8|$$R(c) \wedge S(C)$$ for arbitrary c|Conjunction from (6) and (7)|
|9|$$\forall x (R(x) \wedge S(x))$$|Universal generalization from (8)| 