Show that the argument form with $$(p \wedge t) \rightarrow (r \vee s), q \rightarrow (u \wedge t), u \rightarrow p$$, and $$\neg s$$ and conclusion $$q \rightarrow r$$ is valid by first using Exercise 11 and then using rules of inference from Table 1.

Solution

|Step|Expression|Reason|
|--|--|--|
|1|q|Premise|
|2|$$q \rightarrow (u \wedge t)$$|Premise|
|3|$$u \wedge t$$|Modus ponens from (1) and (2)|
|4|u|Simplification from (3)|
|5|t|Simplification from (3)|
|6|$$u \rightarrow p$$|Premise|
|7|p|Modus ponens from (4) and (6)|
|8|$$p \wedge t$$|Conjunction from (5) and (7)|
|9|$$(p \wedge t) \rightarrow (r \vee s)$$|Premise|
|10|$$r \vee s$$|Modus ponens from (8) and (9)|
|11|$$\neg s$$|Premise|
|12|r|Disjunctive syllogism|

By Exercise 11 $$q \rightarrow r$$ is valid.