Identify the error or errors in this argument that supposedly shows that if $$\exist x P(x) \wedge \exist x Q(x)$$ is true then $$\exist x (P(x) \wedge Q(x))$$ is true.

|Step|Expression|Reason|
|--|--|--|
|1|$$\exist x P(x) \wedge \exist x Q(x)$$|Premise|
|2|$$\exist x P(x)|Simplification from (1)|
|3|P(c)|Existential instantiation from (2)|
|4|$$\exist x Q(x)|Simplification from (1)|
|5|Q(c)|Existential instantiation from (4)|
|6|$$P(c) \wedge Q(c)$$|Conjunction from (3) and (5)|
|7|$$\exist x (P(x) \wedge Q(x))$$|Existential generalization|

Solution

Step 3 and Step 5 may be has two different c.