Explain, without using a truth table, why $$(p \vee q \vee r) \wedge (\neg p \vee \neg q \vee \neg r) is true when at least one of p, q, and r is true and at least one is false, but is false when all three variables have the same truth value.

Solution

1. $$p \vee q \vee r$$ = T
2. $$\neg p \vee \neg q \vee \neg r$$ = T

Equation 1 is T if and only if at least one of p, q, and r is true.

Equation 2 is T if and only if at least one of p, q, and r is false.

Refer: The first clause is true if and only if at least one of p, q, and r is true. The second clause is true if and only if at least one of the three variables is false. Therefore, the entire statement truth values of the variables, in other words, that they don't all have the same truth value.