1. Show that $$\forall x P(x) \wedge \exist x Q(x)$$ is logically equivalent to $$\forall x \exist y (P(x) \wedge Q(y))$$, where all quantifiers have the same nonempty domain.
2. Show that $$\forall P(x) \vee \exist x Q(x)$$ is equivalent to $$\forall x \exist y (P(x) \vee Q(y))$$, where all quantifiers have the same nonempty domain.

a. Assign domain consist of $$x_1, x_2,..., x_n$$

$$\begin{aligned}
\forall x P(x) \wedge \exist x Q(x) 
&\equiv \bigwedge_{i=1}^n P(x_i) \wedge \bigvee_{j=1}^n Q(x_j) \\
&\equiv \bigwedge_{i=1}^n (P(x_i) \wedge \bigvee_{j=1}^n Q(x_j)) \\
&\equiv \bigwedge_{i=1}^n \bigvee_{j=1}^n (P(x_i) \wedge Q(x_j) \\
&\equiv \forall x \exist y (P(x) \wedge Q(y))
\end{aligned}$$

b. Assign domain consist of $$x_1, x_2, ..., x_n$$

$$\begin{aligned}
\forall x P(x) \vee \exist x Q(x) 
&\equiv \bigwedge_{i=1}^n P(x_i) \vee \bigvee_{j=1}^n Q(x_j) \\
&\equiv \bigwedge_{i=1}^n (P(x_i) \vee \bigvee_{j=1}^n Q(x_j)) \\
&\equiv \bigwedge_{i=1}^n \bigvee_{j=1}^n (P(x_i) \vee Q(x_j)) \\
&\equiv \forall x \exist y (P(x) \vee Q(x))
\end{aligned}$$

<style type="text/css">
    ol { list-style-type: lower-alpha; }
</style>