Explain, without using a truth table, why $$(p \vee \neg q) \wedge (q \vee \neg r) \wedge (r \vee \neg p) is true when p, q, and r have the same truth value and it is false otherwise.

Solution

1. $$p \vee \neg q$$ = T
1. $$q \vee \neg r$$ = T
1. $$r \vee \neg p$$ = T

if p = T, then $$\neg p$$ = F, for equation 3, r = T, the same with p, q = T, so p, q, and r have the same truth value T.

if p = F, for equation 1, $$\neg q$$ = T, q = F, the same with p, r = F, so p, q, and r have the same truth value F.