Use rules of inference to show that if $$\forall x (P(x) \vee Q(x))$$ and $$\forall ((\neg P(x) \wedge Q(x)) \rightarrow R(x))$$ are true, then $$\forall x (\neg R(x) \rightarrow P(x))$$ is also true, where the domains of all quantifiers are the same.

Solution

|Step|Expression|Reason|
|--|--|--|
|1|$$\forall x (P(x) \vee Q(x))$$|Premise|
|2|$$P(c) \vee Q(c)$$ for arbitrary c|Universal instantiation from (1)|
|3|$$\forall ((\neg P(x) \wedge Q(x)) \rightarrow R(x))$$|Premise|
|4|$$P(c) \vee \neg Q(x) \vee R(x)$$ for arbitrary c|Universal instantiation from (3)|
|5|$$P(c) \vee R(c)$$ for arbitrary c|Resolution from (4)|
|6|$$\forall x (\neg R(x) \rightarrow P(x))$$|Universal generalization from (5)|