Justify the rule of universal transitivity, which states that if $$\forall x (P(x) \rightarrow Q(x))$$ and $$\forall x (Q(x) \rightarrow R(x))$$ are true, then $$\forall x (P(x) \rightarrow R(x))$$ is true, where the domains of all quantifiers are the same.

Solution

|Step|Expression|Reason|
|--|--|--|
|1|$$\forall x (P(x) \rightarrow Q(x))$$|Premise|
|2|$$P(c) \rightarrow Q(c)$$ for arbitrary c|Universal instantiation|
|3|$$\forall x (Q(x) \rightarrow R(x))$$|Premise|
|4|$$Q(c) \rightarrow R(c)$$ for arbitrary c|Universal instantiation|
|5|$$P(c) \rightarrow R(c)$$ for arbitrary c|Modus ponens|
|6|$$\forall x (P(x) \rightarrow R(x))$$|Universal generalization|