Use rules of inference to show that if $$\forall x (P(x) \vee Q(x))$$, $$\forall x (\neg Q(x) \vee S(x))$$, $$\forall x (R(x) \rightarrow \neg S(x))$$, and $$\exist x \neg P(x)$$ are true, then $$\exist x \neg R(x)$$ is true.

Solution

|Step|Expression|Reason|
|--|--|--|
|1|$$\exist x \neg P(x)$$|Premise|
|2|$$\neg P(c)$$|Existential instantiation from (1)|
|3|$$\forall x (P(x) \vee Q(x))$$|Premise|
|4|$$P(c) \vee Q(c)$$|Universal instantiation from (3)|
|5|Q(c)|Disjunctive syllogism from (2) and (4)|
|6|$$\forall x (\neg Q(x) \vee S(x))$$|Premise|
|7|$$Q(c) \rightarrow S(c)$$|Universal instantiation from (6)|
|8|S(c)|Modus ponens from (5) and (7)|
|9|$$\forall x (R(x) \rightarrow \neg S(x))$$|Premise|
|10|$$R(c) \rightarrow \neg S(c)|Universal instantiation from (9)|
|11|$$\neg R(c)$$|Modus tollens from (8) and (10)|
|12|$$\exist x \neg R(x)$$|Existential generalization from (11)|