Show that $$(p \rightarrow q) \rightarrow r$$ and $$p \rightarrow (q \rightarrow r)$$ are not logically equivalent.

Solution

$$\begin{aligned}
(p \rightarrow q) \rightarrow r 
&\equiv \neg [(\neg p \vee q)] \vee r \\
&\equiv (p \wedge \neg q) \vee r \\
&\equiv (p \vee r) \wedge (\neg q \vee r)
\end{aligned}$$

$$\begin{aligned}
p \rightarrow (q \rightarrow r)
&\equiv \neg p \vee (\neg q \vee r)
\end{aligned}$$

when 
$$\begin{cases}
p = F \\
r = F
\end{cases}$$ they has different truth value.