Show that $$(p \wedge q) \rightarrow r$$ and $$(p \rightarrow r) \wedge (q \rightarrow r)$$ are not logically equivalent.

Solution

$$\begin{aligned}
(p \wedge q) \rightarrow r 
&\equiv \neg (p \wedge q) \vee r \\
&\equiv \neg p \vee \neg q \vee r
\end{aligned}$$

$$\begin{aligned}
(p \rightarrow r) \wedge (q \rightarrow r) 
&\equiv (\neg p \vee r) \wedge (\neg q \vee r) \\
&\equiv (\neg p \wedge \neg q) \vee r
\end{aligned}$$

when
$$\begin{cases}
p = T \\
q = F \\
r = F
\end{cases}$$ they has different truth value.