Show that $$(p \rightarrow q) \rightarrow (r \rightarrow s)$$ and $$(p \rightarrow r) \rightarrow (q \rightarrow s)$$ are not logically equivalent.

Solution

$$\begin{aligned}
(p \rightarrow q) \rightarrow (r \rightarrow s)
&\equiv \neg (p \rightarrow q) \vee (r \rightarrow s) \\
&\equiv \neg (\neg p \vee q) \vee (\neg r \vee s) \\
&\equiv (p \wedge \neg q) \vee \neg r \vee s \\
&\equiv [(p \vee \neg r) \wedge (\neg q \vee \neg r)] \vee s
\end{aligned}$$


$$\begin{aligned}
(p \rightarrow r) \rightarrow (q \rightarrow s)
&\equiv \neg (p \rightarrow r) \vee (q \rightarrow s) \\
&\equiv \neg (\neg p \vee r) \vee (\neg q \vee s) \\
&\equiv (p \wedge \neg r) \vee \neg q \vee s \\
&\equiv [(p \vee \neg q) \wedge (\neg r \vee \neg q)] \vee s
\end{aligned}$$

when
$$\begin{cases}
p = F \\
q = T \\
r = F \\
s = F
\end{cases}$$ they has different truth value.