The **dual** of a compound proposition that contains only the logical operations $$\vee$$, $$\wedge$$, and $$\neg$$ is the compound proposition obtained by replacing each $$\vee$$ by $$\wedge$$, each $$\wedge$$ by $$\vee$$, each T by F, and each F by T. The dual of s is denoted by $$s^*$$

**38.** Find the dual of each of these compound propositions.

1. $$p \vee \neg q$$
2. $$p \wedge (q \vee (r \wedge T))$$
3. $$(p \wedge \neg q) \vee (q \wedge F)$$

Solution

1. $$s^* = p \wedge \neg q$$
2. $$s^* = p \vee (q \wedge (r \vee F))$$
3. $$s^* = (p \vee \neg q) \wedge (q \vee T)$$

**39.** Find the dual of each of these compound propositions.

1. $$p \wedge \neg q \wedge \neg r$$
2. $$(p \wedge q \wedge r) \vee s$$
3. $$(p \vee F) \wedge (q \vee T)$$

Solution

1. $$s^* = p \vee \neg q \vee \neg r$$
2. $$s^* = (p \vee q \vee r) \wedge s$$
3. $$s^* = (p \wedge T) \vee (q \wedge F)$$

<style type="text/css">
    ol { list-style-type: lower-alpha; }
</style>