Show that $$(p \rightarrow q) \wedge (q \rightarrow r) \rightarrow (p \rightarrow r)$$ is a tautology.

Solution

$$\begin{aligned}
(p \rightarrow q) \wedge (q \rightarrow r) \rightarrow (p \rightarrow r) 
&\equiv \neg [(p \rightarrow q) \wedge (q \rightarrow r)] \vee (p \rightarrow r) \\
&\equiv \neg [(\neg p \vee q) \wedge (\neg q \vee r)] \vee (\neg p \vee r) \\
&\equiv (p \wedge \neg q) \vee \neg p \vee (q \wedge \neg r) \vee r \\
&\equiv [(p \vee \neg p) \wedge (\neg q \vee \neg p)] \vee [(q \vee r) \wedge (\neg r \vee r)] \\
&\equiv \neg q \vee \neg p \vee q \vee r \\
&\equiv T \vee \neg p \vee r \\
&\equiv T
\end{aligned}$$