Rewrite each of these statements so that negations appear only within predicates (that is , so that no negation is outside a quantifier or an expression involving logical connectives).

1. $$\neg \forall x \forall y P(x, y)$$
2. $$\neg \forall y \exist x P(x, y)$$
3. $$\neg \forall y \forall x (P(x, y) \vee Q(x, y))$$
4. $$\neg (\exist x \exist y \neg P(x, y) \wedge \forall x \forall y Q(x, y))$$
5. $$\neg \forall x (\exist y \forall z P(x, y, z) \wedge \exist z \forall y P(x, y, z))$$

Solution

1. $$\exist x \exist y \neg P(x, y)$$
2. $$\exist y \forall x \neg P(x, y)$$
3. $$\exist y \exist x (\neg P(x, y) \wedge \neg Q(x, y))$$
4. $$(\forall x \forall y P(x, y) \vee \exist x \exist y \neg Q(x, y))$$
5. $$\exist x (\forall y \exist z \neg P(x, y, z) \vee \forall z \exist y \neg P(x, y, z))$$


<style type="text/css">
    ol { list-style-type: lower-alpha; }
</style>