Express the negations of each of these statements so that all negation symbols immediately precede predicates.

1. $$\forall x \exist y \forall z T(x, y, z)$$
2. $$\forall x \exist y P(x, y) \vee \forall x \exist y Q(x, y)$$
3. $$\forall x \exist y (P(x, y) \wedge \exist z R(x, y, z))$$
4. $$\forall x \exist y (P(x, y) \rightarrow Q(x, y))$$

Solution

1. $$\exist x \forall y \exist z \neg T(x, y, z)$$
2. $$\exist x \forall y \neg P(x, y) \wedge \exist x \forall y \neg Q(x, y)$$
3. $$\exist x \forall y (\neg P(x, y) \vee \forall z \neg R(x, y, z))$$
4. $$\exist x \forall y (P(x, y) \wedge \neg Q(x, y))$$


<style type="text/css">
    ol { list-style-type: lower-alpha; }
</style>