Rewrite each of these statements so that negations appear only within predicates (that is, so that no negation is outside a quantifier or an expression involving logical connectives).

1. $$\neg \exist y \exist x P(x, y)$$
2. $$\neg \forall x \exist y P(x, y)$$
3. $$\neg \exist y (Q(y) \wedge \forall x \neg R(x, y))$$
4. $$\neg \exist y (\exist x R(x, y) \vee \forall x S(x, y))$$
5. $$\neg \exist y (\forall x \exist z T(x, y, z) \vee \exist x \forall z U(x, y, z))$$

Solution

1. $$\forall y \forall x \neg P(x, y)$$
2. $$\exist x \forall y \neg P(x, y)$$
3. $$\forall y (\neg Q(x) \vee \exist x R(x, y))$$
4. $$\forall y (\forall x \neg R(x, y) \wedge \exist x \neg S(x, y))$$
5. $$\forall y (\exist x \forall z \neg T(x, y,z) \wedge \forall x \exist z \neg U(x, y,z))$$


<style type="text/css">
    ol { list-style-type: lower-alpha; }
</style>