Show that $$\forall x P(x) \wedge \forall x Q(x)$$ and $$\forall x \forall y (P(x) \wedge Q(y))$$ where all quantifiers have the same nonempty domain, are logically equivalent. (The new variable y is used to combine the quantifications correctly.)

Solution

Assign domain consist of $$x_1, x_2, ..., x_n$$

$$\begin{aligned}
\forall x \forall y (P(x) \wedge Q(y)) 
&\equiv \bigwedge_{i=1}^n \bigwedge_{j=1}^n (P(x_i) \wedge Q(x_j)) \\
&\equiv \bigwedge_{i=1}^n \bigwedge_{j=1}^n P(x_i) \wedge \bigwedge_{i=1}^n \bigwedge_{j=1}^n Q(x_j) \\
&\equiv \bigwedge_{i=1}^n P(x_i) \wedge \bigwedge_{j=1}^n Q(x_j) \\
&\equiv \forall x P(x) \wedge \forall Q(x) 
\end{aligned}$$