Express the negations of each of these statements so that all negation symbols immediately precede predicates. 

1. $$\exist z \forall y \forall x T(x, y, z)$$
2. $$\exist x \exist y P(x, y) \wedge \forall x \forall y Q(x, y)$$
3. $$\exist x \exist y (Q(x, y) \leftrightarrow Q(y, x))$$
4. $$\forall y \exist x \exist z (T(x, y, z) \vee Q(x, y))$$

Solution

1. $$\forall z \exist y \exist x \neg T(x, y, z)$$
2. $$\forall x \forall y \neg P(x, y) \vee \exist x \exist y \neg Q(x, y)$$
3. $$\exist x \exist y ((Q(x, y) \wedge \neg Q(y, x)) \vee (\neg Q(x, y) \wedge Q(y, x)))$$
4. $$\exist y \forall x \forall z (\neg T(x, y, z) \wedge \neg Q(x, y))$$


<style type="text/css">
    ol { list-style-type: lower-alpha; }
</style>
