Show that each conditional statement in Exercise 12 is a tautology using the fact that a conditional statement is false exactly when the hypothesis is true and the conclusion is false. (Do not use truth tables.)

a. $$[\neg p \wedge (p \vee q)] \rightarrow q$$

Assign $$[\neg p \wedge (p \vee q)] \rightarrow q = F => \begin{cases}\neg p \wedge (p \vee q) = T \\
q = F \end{cases}$$ conflict.

b. $$[(p \rightarrow q) \wedge (q \rightarrow r)] \rightarrow (p \rightarrow r)$$

Assign $$[(p \rightarrow q) \wedge (q \rightarrow r)] \rightarrow (p \rightarrow r) = F => \begin{cases} (p \rightarrow q) \wedge (q \rightarrow r) = T \\
p \rightarrow r = F \end{cases} => \begin{cases} p \rightarrow q = T \\ 
q \rightarrow r = T \\
p = T\\
r = F \end{cases}$$ conflict.

c. $$[p \wedge (p \rightarrow q)] \rightarrow q$$

Assign $$[p \wedge (p \rightarrow q)] \rightarrow q = T => \begin{cases} p \wedge (p \rightarrow q) = T \\
q = F \end{cases} => \begin{cases} p = T \\
p \rightarrow q = T \\
q = F \end{cases}$$ conflict.

d. $$[(p \vee q) \wedge (p \rightarrow r) \wedge (q \rightarrow r)] \rightarrow r$$

Assign $$[(p \vee q) \wedge (p \rightarrow r) \wedge (q \rightarrow r)] \rightarrow r = F => \begin{cases} (p \vee q) \wedge (p \rightarrow r) \wedge (q \rightarrow r) = T \\
r = F \end{cases} => \begin{cases} p \vee q = T \\
p \rightarrow r = T \\
q \rightarrow r = T \\
r = F \end{cases}$$ conflict.