Show that each of these conditional statements is a tautology by using truth tables.

1. $$(p \wedge q) \rightarrow p$$
2. $$p \rightarrow (p \vee q)$$
3. $$\neg p \rightarrow (p \rightarrow q)$$
4. $$(p \wedge q) \rightarrow (p \rightarrow q)$$
5. $$\neg (p \rightarrow q) \rightarrow p$$
6. $$\neg (p \rightarrow q) \rightarrow \neg q$$

Solution

a. $$(p \wedge q) \rightarrow p$$

|p|q|$$p \wedge q$$|$$p \wedge q) \rightarrow p$$
|--|--|--|--|
|T|T|T|T|
|T|F|F|T|
|F|T|F|T|
|F|F|F|T|

b. $$p \rightarrow (p \vee q)$$

|p|q|$$p \vee q$$|$$p \rightarrow (p \vee q)$$|
|--|--|--|--|
|T|T|T|T|
|T|F|T|T|
|F|T|T|T|
|F|F|F|T|

c. $$\neg p \rightarrow (p \rightarrow q)$$

|p|q|$$\neg p$$|$$p \rightarrow q$$|$$\neg p \rightarrow (p \rightarrow q)$$|
|--|--|--|--|--|
|T|T|F|T|T|
|T|F|F|F|T|
|F|T|T|T|T|
|F|F|T|T|T|

d. $$(p \wedge q) \rightarrow (p \rightarrow q)$$

|p|q|$$p \wedge q$$|$$p \rightarrow q$$|$$(p \wedge q) \rightarrow (p \rightarrow q)$$|
|--|--|--|--|--|
|T|T|T|T|T|
|T|F|F|F|T|
|F|T|F|T|T|
|F|F|F|T|T|

e. $$\neg (p \rightarrow q) \rightarrow p$$

|p|q|$$p \rightarrow q$$|$$\neg (p \rightarrow q)$$|$$\neg (p \rightarrow q) \rightarrow p$$|
|--|--|--|--|--|
|T|T|T|F|T|
|T|F|F|T|T|
|F|T|T|F|T|
|F|F|T|F|T|

f. $$\neg (p \rightarrow q) \rightarrow \neg q$$

|p|q|$$p \rightarrow q$$|$$\neg (p \rightarrow q)$$|$$\neg q$$|$$\neg (p \rightarrow q) \rightarrow \neg q$$|
|--|--|--|--|--|
|T|T|T|F|F|T|
|T|F|F|T|T|T|
|F|T|T|F|F|T|
|F|F|T|F|T|T|

<style type="text/css">
    ol { list-style-type: lower-alpha; }
</style>