For each of these compound propositions, use the conditional-disjunction equivalence (Example 3) to find an equivalent compound proposition that does involve conditionals.

1. $$\neg p \rightarrow \neg q$$
2. $$(p \vee q) \rightarrow \neg p$$
3. $$(p \rightarrow \neg q) \rightarrow (\neg p \rightarrow q)$$

Solution 

1. $$p \vee \neg q$$
2. $$(\neg p \wedge \neg q) \vee \neg p$$
3. $$(p \wedge q) \vee (p \vee q)$$

**Conditional-disjuction equivalence: $$p \rightarrow q \equiv \neg p \vee q$$**

1. $$\neg p \rightarrow \neg q \equiv p \vee \neg q$$
2. $$(p \vee q) \rightarrow \neg p \equiv \neg (p \vee q) \vee \neg p \equiv (\neg p \wedge \neg q) \vee \neg p$$
3. $$(p \rightarrow \neg q) \rightarrow (\neg p \rightarrow q) \equiv \neg (p \rightarrow \neg q) \vee (\neg p \rightarrow q) \equiv \neg (\neg p \vee \neg q) \vee (p \vee q) \equiv (p \wedge q) \vee (p \vee q)$$

<style type="text/css">
    ol { list-style-type: lower-alpha; }
</style>