Show that $$(p \vee q) \wedge (\neg p \vee r) \rightarrow (q \vee r)$$ is a tautology.

Solution

$$\begin{aligned}
(p \vee q) \wedge (\neg p \vee r) \rightarrow (q \vee r) 
&\equiv \neg [(p \vee q) \wedge (\neg p \vee r)] \vee (q \vee r) \\
&\equiv (\neg p \wedge \neg q) \vee q \vee (p \wedge \neg r) \vee r \\
&\equiv [(\neg p \vee q) \wedge (\neg q \vee q)] \vee [(p \vee r) \wedge (\neg r \vee r)] \\
&\equiv \neg p \vee q \vee p \vee r \\
&\equiv T \vee q \vee r \\
&\equiv T
\end{aligned}$$