Show that each conditional statement in Exercise 11 is a tautology using the fact that a conditional statement is false exaclty when the hypothesis is true and the conclusion is false. (Do not use truth tables.)

Solution

a. $$(p \wedge q) \rightarrow p$$

Assign $$(p \wedge q) \rightarrow p = F => \begin{cases} p \wedge q = T \\
p = F \end{cases}$$ confilict.

b. $$p \rightarrow (p \vee q)$$

Assign $$p \rightarrow (p \vee q) = F => \begin{cases} p = T \\
p \vee q = F \end{cases}$$ confilict.

c. $$\neg p \rightarrow (p \rightarrow q)$$

Assign $$\neg p \rightarrow (p \rightarrow q) = F => \begin{cases} \neg p = T \\
p \rightarrow q = F \end{cases}$$ conflict.

d. $$(p \wedge q) \rightarrow (p \rightarrow q)$$

Assign $$(p \wedge q) \rightarrow (p \rightarrow q) = F => \begin{cases} p \wedge q = T \\
p \rightarrow q = F \end{cases}$$ conflict.

e. $$\neg (p \rightarrow q) \rightarrow p$$

Assign $$\neg (p \rightarrow q) \rightarrow p = F => \begin{cases} \neg (p \rightarrow q) = T \\
p = F \end{cases}$$ conflict.

f. $$\neg (p \rightarrow q) \rightarrow \neg q$$

Assign $$\neg (p \rightarrow q) \rightarrow \neg q = F => \begin{cases} \neg (p \rightarrow q) = T \\
\neg q = F \end{cases} = > \begin{cases} p = T \\
q = F\\
\neg q = F \end{cases}$$ conflict.