Show that each conditional statement in Exercise 11 is a tautology by applying achain of logical identities as in Example 8. (Do not use truth tables.)

Solution

**a. $$(p \wedge q) \rightarrow p$$**

$$\begin{aligned}
(p \wedge q) \rightarrow p 
&\equiv \neg (p \wedge q) \vee p \\
&\equiv (\neg p \vee \neg q) \vee p \\
&\equiv T \vee \neg q \\ 
&\equiv T \end{aligned}$$

**b. $$p \rightarrow (p \vee q)$$**

$$\begin{aligned}
p \rightarrow (p \vee q) 
&\equiv \neg p \vee (p \vee q) \\
&\equiv T \vee q \\
&\equiv T \end{aligned}$$

**c. $$\neg p \rightarrow (p \rightarrow q)$$**

$$\begin{aligned}
\neg p \rightarrow (p \rightarrow q) 
&\equiv \neg (\neg p) \vee (p \rightarrow q) \\
&\equiv p \vee (\neg p \vee q) \\
&\equiv T \vee q \\
&\equiv T \end{aligned}$$

**d. $$(p \wedge q) \rightarrow (p \rightarrow q)$$**

$$\begin{aligned}
(p \wedge q) \rightarrow (p \rightarrow q) 
&\equiv \neg (p \wedge q) \vee (p \rightarrow q) \\
&\equiv \neg p \vee \neg q \vee (\neg p \vee q) \\
&\equiv \neg p \vee T \\
&\equiv T \end{aligned}$$

**e. $$\neg (p \rightarrow q) \rightarrow p$$**

$$\begin{aligned}
\neg (p \rightarrow q) \rightarrow p 
&\equiv \neg (\neg (p \rightarrow q)) \vee p \\
&\equiv \neg p \vee q \vee p \\
&\equiv T \vee q \\
&\equiv T \end{aligned}$$

**f. $$\neg (p \rightarrow q) \rightarrow \neg q$$**

$$\begin{aligned}
\neg (p \rightarrow q) \rightarrow \neg q 
&\equiv \neg (\neg (p \rightarrow q) \vee \neg q \\
&\equiv \neg p \vee q \vee \neg q \\
&\equiv \neg p \vee T \\
&\equiv T \end{aligned}$$