For each of these compoound propositions, use the conditional-disjunction equivalence (Example 3) to find an equivalent compound proposition that does not involue conditionals.

1. $$p \rightarrow \neg q$$
2. $$(p \rightarrow q) \rightarrow r$$
3. $$(\neg q \rightarrow p) \rightarrow (p \rightarrow \neg q)$$

Solution

1. $$\neg p \vee \neg q$$
2. $$(p \wedge \neg q) \vee r$$
3. $$(\neg p \wedge \neg q) \vee (\neg p \vee \neg q)$$


**Conditional-disjuction equivalence: $$p \rightarrow q \equiv \neg p \vee q$$**

1. $$p \rightarrow \neg q \equiv \neg p \vee \neg q$$
2. $$(p \rightarrow q) \rightarrow r \equiv \neg (p \rightarrow q) \vee \neg r \equiv \neg (\neg p \vee q) \vee r \equiv (p \wedge \neg q) \vee r$$
3. $$(\neg q \rightarrow p) \rightarrow (p \rightarrow \neg q) \equiv \neg (\neg q \rightarrow p) \vee (p \rightarrow \neg q) \equiv \neg (q \vee p) \vee (\neg p \vee \neg q) \equiv (\neg p \wedge \neg q) \vee (\neg p \vee \neg q)$$


<style type="text/css">
    ol { list-style-type: lower-alpha; }
</style>