Use truth tables to verify the absorption laws.

1. $$p \vee (p \wedge q) \equiv p$$
2. $$p \wedge (p \vee q) \equiv p$$

Solution

a. $$p \vee (p \wedge q) \equiv p$$

|p|q|$$p \wedge q$$|$$p \vee (p \wedge q)$$|
|--|--|--|--|
|T|T|T|T|
|T|F|F|T|
|F|T|F|F|
|F|F|F|F|

b. $$p \wedge (p \vee q) \equiv p$$

|p|q|$$p \vee q$$|$$p \wedge (p \vee q)$$|
|--|--|--|--|
|T|T|T|T|
|T|F|T|T|
|F|T|T|F|
|F|F|F|F|

<style type="text/css">
    ol { list-style-type: lower-alpha; }
</style>