Show that each conditional statement in Exercise 12 is a tautology by applying a chain of logical identities as in Example 8. (Do not use truth tables.) 

Solution

**a. $$[\neg p \wedge (p \vee q)] \rightarrow q$$**

$$\begin{aligned}
[\neg p \wedge (p \vee q)] \rightarrow q 
&\equiv \neg (\neg p \wedge (p \vee q)) \vee q \\
&\equiv p \vee \neg (p \vee q) \vee q \\
&\equiv (p \vee q) \vee \neg (p \vee q) \\
&\equiv T \end{aligned}$$

**b. $$[(p \rightarrow q) \wedge (q \rightarrow r)] \rightarrow (p \rightarrow r)$$**

$$\begin{aligned}
[(p \rightarrow q) \wedge (q \rightarrow r)] \rightarrow (p \rightarrow r) 
&\equiv \neg ((p \rightarrow q) \wedge (q \rightarrow r)) \vee (p \rightarrow r) \\ 
\\
&\equiv \neg ((\neg p \vee q) \wedge (\neg q \vee r)) \vee (\neg p \vee r) \\
\\
&\equiv \neg (\neg p \vee q) \vee \neg (\neg q \vee r) \vee (\neg p \vee r) \\
&\equiv (p \wedge \neg q) \vee (q \wedge \neg r) \vee (\neg p \vee r) \\
&\equiv [(p \wedge \neg q) \vee \neg p] \vee [(q \wedge \neg r) \vee r] \\
&\equiv [(p \vee \neg p) \wedge (\neg q \vee \neg p)] \vee [(q \vee r) \wedge (\neg r \vee r)] \\
&\equiv \neg q \vee \neg p \vee q \vee r \\
&\equiv T \vee \neg p \vee r \\
&\equiv T \end{aligned}$$

**c. $$[p \wedge (p \rightarrow q)] \rightarrow q$$**

$$\begin{aligned}
[p \wedge (p \rightarrow q)] \rightarrow q 
&\equiv \neg [p \wedge (p \rightarrow q)] \vee q \\
&\equiv \neg p \vee (\neg p \vee q) \vee q \\
&\equiv T \vee q \\
&\equiv T \end{aligned}$$

**d. $$[(p \vee q) \wedge (p \rightarrow r) \wedge (q \rightarrow r)] \rightarrow r$$**

$$\begin{aligned}
[(p \vee q) \wedge (p \rightarrow r) \wedge (q \rightarrow r)] \rightarrow r 
&\equiv \neg [(p \vee q) \wedge (p \rightarrow r) \wedge (q \rightarrow r)] \vee r \\
&\equiv \neg (p \vee q) \vee \neg (\neg p \vee r) \vee \neg (\neg q \vee r) \vee r \\
&\equiv (\neg p \wedge \neg q) \vee (p \wedge \neg r) \vee [(q \wedge \neg r) \vee r] \\
&\equiv (\neg p \wedge \neg q) \vee (p \wedge \neg r) \vee [(q \vee r) \wedge (\neg r \vee r)] \\
&\equiv (\neg p \wedge \neg q) \vee (p \wedge \neg r) \vee (q \vee r) \\
&\equiv [(\neg p \wedge \neg q) \vee q] \vee [(p \wedge \neg r) \vee r] \\
&\equiv [(\neg p \vee q) \wedge (\neg q \vee q)] \vee [(p \vee r) \wedge (\neg r \vee r)] \\
&\equiv (\neg p \vee q) \vee (p \vee r) \\
&\equiv T \vee q \vee r \\
&\equiv T \end{aligned}$$